Lem.dfy
@@ -1,0 +1,42 @@
+include "Type.dfy"
+include "Property.dfy"
+module Lem {
+  import opened Type
+  import opened Property
+
+  function makeRootBlack(t: Rb_tree): Rb_tree
+  {
+    match t
+    case Node(_, k, l, r) => Node(Black, k, l, r)
+    case Null => Null
+  }
+
+  lemma lem_make_black (t:Rb_tree)
+    ensures root_property2(makeRootBlack(t)) {
+  }
+
+  lemma bst_meaning(t:Rb_tree)
+    requires t.Node? &&t.left.Node? && t.right.Node? && bst_property(t)
+    ensures t.left.key < t.key
+    ensures t.right.key > t.key
+  {
+    assert t.left.key in contain(t.left);
+    assert forall x :: x in contain(t.left) ==> x < t.key;
+    assert t.left.key < t.key;
+
+    assert t.right.key in contain(t.right);
+    assert forall x :: x in contain(t.right) ==> x > t.key;
+    assert t.right.key > t.key;
+  }
+  lemma bst_transitivity_right(t:Rb_tree)
+    requires t.Node? &&t.left.Node? && t.right.Node? && bst_property(t)
+    ensures forall x :: x in contain (t.left.right)==> x < t.key
+
+  {
+    assert bst_property(t);
+    assert bst_property(t.left);
+    assert bst_property(t.right);
+    assert forall x :: x in contain(t.left.right) ==> x in contain(t.left);
+
+  }
+}
